Add proofs for eBPF-backend

ebpf/NeedOp.v
@@ -10,11 +10,71 @@
 (*                                                                     *)
 (* *********************************************************************)
 
-Require Import Op.
+Require Import Coqlib.
+Require Import AST Integers Floats.
+Require Import Values Memory Globalenvs.
+Require Import Op RTL.
 Require Import NeedDomain.
 
 Definition needs_of_condition (cond: condition): list nval := nil.
 
 Definition needs_of_operation (op: operation) (nv: nval): list nval := nil.
 
-Definition operation_is_redundant (op: operation) (nv: nval): bool := false.
+Definition operation_is_redundant (op: operation) (nv: nval): bool :=
+  match op with
+  | Omove | _ => false
+  end.
+
+Ltac InvAgree :=
+  match goal with
+  | [H: vagree_list nil _ _ |- _ ] => inv H; InvAgree
+  | [H: vagree_list (_::_) _ _ |- _ ] => inv H; InvAgree
+  | _ => idtac
+  end.
+
+Ltac TrivialExists :=
+  match goal with
+  | [ |- exists v, Some ?x = Some v /\ _ ] => exists x; split; auto
+  | _ => idtac
+  end.
+
+Section SOUNDNESS.
+
+Variable ge: genv.
+Variable sp: block.
+Variables m m': mem.
+Hypothesis PERM: forall b ofs k p, Mem.perm m b ofs k p -> Mem.perm m' b ofs k p.
+
+Lemma needs_of_condition_sound:
+  forall cond args b args',
+  eval_condition cond args m = Some b ->
+  vagree_list args args' (needs_of_condition cond) ->
+  eval_condition cond args' m' = Some b.
+Proof.
+  intros. unfold needs_of_condition in H0.
+  eapply default_needs_of_condition_sound; eauto.
+Qed.
+Lemma needs_of_operation_sound:
+  forall op args v nv args',
+  eval_operation ge (Vptr sp Ptrofs.zero) op args m = Some v ->
+  vagree_list args args' (needs_of_operation op nv) ->
+  nv <> Nothing ->
+  exists v',
+     eval_operation ge (Vptr sp Ptrofs.zero) op args' m' = Some v'
+  /\ vagree v v' nv.
+Proof.
+  unfold needs_of_operation; intros; destruct op; try (eapply default_needs_of_operation_sound; eauto; fail);
+  simpl in *; FuncInv; InvAgree; TrivialExists.
+Qed.
+
+Lemma operation_is_redundant_sound:
+  forall op nv arg1 args v arg1' args',
+  operation_is_redundant op nv = true ->
+  eval_operation ge (Vptr sp Ptrofs.zero) op (arg1 :: args) m = Some v ->
+  vagree_list (arg1 :: args) (arg1' :: args') (needs_of_operation op nv) ->
+  vagree v arg1' nv.
+Proof.
+  intros. destruct op; simpl in *; try discriminate; inv H1; FuncInv; subst.
+Qed.
+
+End SOUNDNESS.
